Using arbitrary tactic

src/cdcl.ml
@@ -2,6 +2,8 @@ open Names
 open Constr
 module P = ProverPatch
 
+let pr_constr env evd e = Printer.pr_econstr_env env evd e
+
 let constr_of_gref r =
   EConstr.of_constr (UnivGen.constr_of_monomorphic_global r)
 
@@ -10,6 +12,16 @@ let coq_True = lazy (Coqlib.lib_ref "core.True.type")
 let coq_False = lazy (Coqlib.lib_ref "core.False.type")
 let coq_and = lazy (Coqlib.lib_ref "core.and.type")
 let coq_or = lazy (Coqlib.lib_ref "core.or.type")
+let coq_true = lazy (Coqlib.lib_ref "core.bool.true")
+let coq_false = lazy (Coqlib.lib_ref "core.bool.false")
+let coq_orb = lazy (Coqlib.lib_ref "core.bool.orb")
+let coq_andb = lazy (Coqlib.lib_ref "core.bool.andb")
+let coq_implb = lazy (Coqlib.lib_ref "core.bool.implb")
+let coq_Is_true = lazy (Coqlib.lib_ref "cdcl.Is_true")
+let coq_None = lazy (constr_of_ref "core.option.None")
+let coq_Some = lazy (constr_of_ref "core.option.Some")
+let coq_iff_refl = lazy (constr_of_ref "cdcl.iff_refl")
+let coq_nnpp = lazy (constr_of_ref "core.nnpp.type")
 
 (*let coq_iff = lazy (Coqlib.lib_ref "core.iff.type") *)
 
@@ -23,27 +35,53 @@ let coq_AND = lazy (constr_of_ref "cdcl.op.AND")
 let coq_OR = lazy (constr_of_ref "cdcl.op.OR")
 let coq_IMPL = lazy (constr_of_ref "cdcl.op.IMPL")
 let coq_hc = lazy (constr_of_ref "cdcl.HCons.mk")
-let coq_true = lazy (constr_of_ref "core.bool.true")
-let coq_false = lazy (constr_of_ref "core.bool.false")
 let coq_int = lazy (constr_of_ref "num.int63.type")
+
+(* Boolean formula terms *)
+let coq_IsBool = lazy (constr_of_ref "cdcl.kind.IsBool")
+let coq_IsProp = lazy (constr_of_ref "cdcl.kind.IsProp")
+let coq_BFormula = lazy (constr_of_ref "cdcl.BFormula.type")
+let coq_BTT = lazy (constr_of_ref "cdcl.BFormula.BTT")
+let coq_BFF = lazy (constr_of_ref "cdcl.BFormula.BFF")
+let coq_BAT = lazy (constr_of_ref "cdcl.BFormula.BAT")
+let coq_BOP = lazy (constr_of_ref "cdcl.BFormula.BOP")
+let coq_BIT = lazy (constr_of_ref "cdcl.BFormula.BIT")
 
 (* Evaluation *)
 let coq_eval_is_dec = lazy (constr_of_ref "cdcl.eval_is_dec")
-let coq_dProp = lazy (constr_of_ref "cdcl.dProp")
-let coq_DecP1 = lazy (constr_of_ref "cdcl.DecP1")
-let coq_DecP2 = lazy (constr_of_ref "cdcl.DecP2")
-let coq_decP1 = lazy (constr_of_ref "cdcl.decP1")
-let coq_decP2 = lazy (constr_of_ref "cdcl.decP2")
+let coq_atomT = lazy (constr_of_ref "cdcl.atomT.type")
 let coq_mkAtom = lazy (constr_of_ref "cdcl.mkAtom")
-let coq_mkDecAtom = lazy (constr_of_ref "cdcl.mkDecAtom")
+let coq_mkAtomDec = lazy (constr_of_ref "cdcl.mkAtomDec")
+let coq_TBool = lazy (constr_of_ref "cdcl.atomT.TBool")
+let coq_DecP1 = lazy (constr_of_ref "cdcl.DecP1")
+let coq_decP1 = lazy (constr_of_ref "cdcl.decP1")
+let coq_DecP2 = lazy (constr_of_ref "cdcl.DecP2")
+let coq_decP2 = lazy (constr_of_ref "cdcl.decP2")
+let coq_Rbool1 = lazy (constr_of_ref "cdcl.Rbool1.type")
+let coq_p1 = lazy (constr_of_ref "cdcl.Rbool1.p1")
+let coq_p1_prf = lazy (constr_of_ref "cdcl.Rbool1.p1_prf")
+let coq_Rbool2 = lazy (constr_of_ref "cdcl.Rbool2.type")
+let coq_p2 = lazy (constr_of_ref "cdcl.Rbool2.p2")
+let coq_p2_prf = lazy (constr_of_ref "cdcl.Rbool2.p2_prf")
+let coq_RProp1 = lazy (constr_of_ref "cdcl.RProp1.type")
+let coq_b1 = lazy (constr_of_ref "cdcl.RProp1.b1")
+let coq_b1_prf = lazy (constr_of_ref "cdcl.RProp1.b1_prf")
+let coq_RProp2 = lazy (constr_of_ref "cdcl.RProp2.type")
+let coq_b2 = lazy (constr_of_ref "cdcl.RProp2.b2")
+let coq_b2_prf = lazy (constr_of_ref "cdcl.RProp2.b2_prf")
 let coq_eval_prop = lazy (constr_of_ref "cdcl.eval_prop")
 let coq_eval_hformula = lazy (constr_of_ref "cdcl.eval_hformula")
+let coq_eval_hbformula = lazy (constr_of_ref "cdcl.eval_hbformula")
 let coq_empty = lazy (constr_of_ref "cdcl.IntMap.empty")
 let coq_add = lazy (constr_of_ref "cdcl.IntMap.add")
 
 let is_prop env sigma term =
   let sort = Retyping.get_sort_of env sigma term in
   Sorts.is_prop sort
+
+let constr_of_option typ constr_of_val = function
+  | None -> EConstr.mkApp (Lazy.force coq_None, [|typ|])
+  | Some v -> EConstr.mkApp (Lazy.force coq_Some, [|typ; constr_of_val v|])
 
 module IMap = Map.Make (Int)
 
@@ -56,21 +94,29 @@ module Env = struct
 
   module AMap = Map.Make (Int)
 
-  type dec = NotDec | IsDec of EConstr.t (* Proof of p \/ ~ p *)
+  type atom_spec =
+    | AtomProp of EConstr.t * EConstr.t option (* NBool *)
+    | AtomBool of EConstr.t * EConstr.t * EConstr.t
 
-  let is_dec = function NotDec -> false | IsDec _ -> true
+  (* TBool *)
 
   type t =
     { fresh : int
-    ; vars : (EConstr.t * (int * dec)) list (* hcons value for atoms *)
-    ; amap : (EConstr.t * dec) AMap.t (* same as vars + is_dec*)
+    ; vars : (atom_spec * int) list (* hcons value for atoms *)
+    ; amap : atom_spec AMap.t (* same as vars + is_dec*)
     ; hmap : int OMap.t
     ; sigma : Evd.evar_map }
+
+  let get_proposition_of_atom_spec = function
+    | AtomProp (p, _) -> p
+    | AtomBool (_, p, _) -> p
 
   let get_constr_of_atom ep a =
     ProverPatch.(
       match a.HCons.elt with
-      | AT i -> (fst (AMap.find (Uint63.hash i) ep.amap), Uint63.hash i)
+      | AT i ->
+        ( get_proposition_of_atom_spec (AMap.find (Uint63.hash i) ep.amap)
+        , Uint63.hash i )
       | _ -> raise Not_found)
 
   let empty sigma =
@@ -103,8 +149,8 @@ module Env = struct
         let tc = EConstr.mkApp (Lazy.force coq_DecP1, [|ty; c|]) in
         try
           let _evd, dec = Typeclasses.resolve_one_typeclass env evd tc in
-          IsDec (EConstr.mkApp (Lazy.force coq_decP1, [|ty; c; dec; a.(1)|]))
-        with Not_found -> NotDec
+          Some (EConstr.mkApp (Lazy.force coq_decP1, [|ty; c; dec; a.(0)|]))
+        with Not_found -> None
       else
         let c, v1, v2 =
           if len = 2 then (c, a.(0), a.(1))
@@ -118,31 +164,132 @@ module Env = struct
         let tc = EConstr.mkApp (Lazy.force coq_DecP2, [|ty1; ty2; c|]) in
         try
           let _evd, dec = Typeclasses.resolve_one_typeclass env evd tc in
-          IsDec
+          Some
             (EConstr.mkApp (Lazy.force coq_decP2, [|ty1; ty2; c; dec; v1; v2|]))
-        with Not_found -> NotDec )
-    | _ -> NotDec
+        with Not_found -> None )
+    | _ -> None
 
-  let hcons_atom genv env v =
+  let default_bool t =
+    let is_true =
+      EConstr.mkApp (constr_of_gref (Lazy.force coq_Is_true), [|t|])
+    in
+    AtomBool (t, is_true, EConstr.mkApp (Lazy.force coq_iff_refl, [|is_true|]))
+
+  let make_atom_of_bool env evd t =
+    match EConstr.kind evd t with
+    | App (c, a) -> (
+      let len = Array.length a in
+      if len = 1 then
+        (* Unary predicate *)
+        let ty = Retyping.get_type_of env evd a.(0) in
+        let tc = EConstr.mkApp (Lazy.force coq_Rbool1, [|ty; c|]) in
+        try
+          let _evd, refl = Typeclasses.resolve_one_typeclass env evd tc in
+          let p1 = EConstr.mkApp (Lazy.force coq_p1, [|ty; c; refl; a.(0)|]) in
+          let p1_prf =
+            EConstr.mkApp (Lazy.force coq_p1_prf, [|ty; c; refl; a.(0)|])
+          in
+          AtomBool (t, p1, p1_prf)
+        with Not_found -> default_bool t
+      else
+        let c, v1, v2 =
+          if len = 2 then (c, a.(0), a.(1))
+          else
+            ( EConstr.mkApp (c, Array.sub a 0 (Array.length a - 2))
+            , a.(len - 2)
+            , a.(len - 1) )
+        in
+        let ty1 = Retyping.get_type_of env evd v1 in
+        let ty2 = Retyping.get_type_of env evd v2 in
+        let tc = EConstr.mkApp (Lazy.force coq_Rbool2, [|ty1; ty2; c|]) in
+        try
+          let _evd, refl = Typeclasses.resolve_one_typeclass env evd tc in
+          let p2 =
+            EConstr.mkApp (Lazy.force coq_p2, [|ty1; ty2; c; refl; v1; v2|])
+          in
+          let p2_prf =
+            EConstr.mkApp (Lazy.force coq_p2_prf, [|ty1; ty2; c; refl; v1; v2|])
+          in
+          AtomBool (t, p2, p2_prf)
+        with Not_found -> default_bool t )
+    | _ -> default_bool t
+
+  let default_prop env evd t = AtomProp (t, is_dec_constr env evd t)
+
+  let make_atom_of_prop env evd t =
+    match EConstr.kind evd t with
+    | App (c, a) -> (
+      let len = Array.length a in
+      if len = 1 then
+        (* Unary predicate *)
+        let ty = Retyping.get_type_of env evd a.(0) in
+        let tc = EConstr.mkApp (Lazy.force coq_RProp1, [|ty; c|]) in
+        try
+          let _evd, refl = Typeclasses.resolve_one_typeclass env evd tc in
+          let b1 = EConstr.mkApp (Lazy.force coq_b1, [|ty; c; refl; a.(0)|]) in
+          let b1_prf =
+            EConstr.mkApp (Lazy.force coq_b1_prf, [|ty; c; refl; a.(0)|])
+          in
+          AtomBool (b1, t, b1_prf)
+        with Not_found -> default_prop env evd t
+      else
+        let c, v1, v2 =
+          if len = 2 then (c, a.(0), a.(1))
+          else
+            ( EConstr.mkApp (c, Array.sub a 0 (Array.length a - 2))
+            , a.(len - 2)
+            , a.(len - 1) )
+        in
+        let ty1 = Retyping.get_type_of env evd v1 in
+        let ty2 = Retyping.get_type_of env evd v2 in
+        let tc = EConstr.mkApp (Lazy.force coq_RProp2, [|ty1; ty2; c|]) in
+        try
+          let _evd, refl = Typeclasses.resolve_one_typeclass env evd tc in
+          let p2 =
+            EConstr.mkApp (Lazy.force coq_p2, [|ty1; ty2; c; refl; v1; v2|])
+          in
+          let p2_prf =
+            EConstr.mkApp (Lazy.force coq_p2_prf, [|ty1; ty2; c; refl; v1; v2|])
+          in
+          AtomBool (t, p2, p2_prf)
+        with Not_found -> default_prop env evd t )
+    | _ -> default_prop env evd t
+
+  let eq_constr_atom_spec (genv, sigma) k a v =
+    match k with
+    | P.IsProp -> eq_constr (genv, sigma) (get_proposition_of_atom_spec a) v
+    | P.IsBool -> (
+      match a with
+      | AtomProp _ -> None
+      | AtomBool (b, _, _) -> eq_constr (genv, sigma) b v )
+
+  let hcons_atom genv env k v =
     let rec find sigma v vars =
       match vars with
       | [] -> raise Not_found
       | (e, i) :: vars -> (
-        match eq_constr (genv, sigma) e v with
-        | Some sigma' -> (sigma', i)
+        match eq_constr_atom_spec (genv, sigma) k e v with
+        | Some sigma' -> (sigma', (e, i))
         | None -> find sigma v vars )
     in
     try
       let sigma', i = find env.sigma v env.vars in
       ({env with sigma = sigma'}, i)
     with Not_found ->
-      let dec = is_dec_constr genv env.sigma v in
       let f = env.fresh in
+      let atom =
+        match k with
+        | P.IsProp -> make_atom_of_prop genv env.sigma v
+        | P.IsBool -> make_atom_of_bool genv env.sigma v
+      in
       ( { env with
-          vars = (v, (f, dec)) :: env.vars
-        ; amap = AMap.add f (v, dec) env.amap
+          vars = (atom, f) :: env.vars
+        ; amap = AMap.add f atom env.amap
         ; fresh = f + 1 }
-      , (f, dec) )
+      , (atom, f) )
+
+  let is_dec = function AtomProp (_, None) -> false | _ -> true
+  let has_bool = function AtomBool _ -> true | _ -> false
 
   let hcons_op env op f1 f2 =
     try (env, OMap.find (op, f1, f2) env.hmap)
@@ -154,13 +301,14 @@ module Env = struct
 
   let map_of_env env =
     let add = Lazy.force coq_add in
-    let ty = Lazy.force coq_dProp in
-    let mk_atom = Lazy.force coq_mkAtom in
-    let mk_dec_atom = Lazy.force coq_mkDecAtom in
-    let mk_atom (p, d) =
-      match d with
-      | NotDec -> EConstr.mkApp (mk_atom, [|p|])
-      | IsDec prf -> EConstr.mkApp (mk_dec_atom, [|p; prf|])
+    let ty = Lazy.force coq_atomT in
+    let mk_atom a =
+      match a with
+      | AtomProp (p, None) -> EConstr.mkApp (Lazy.force coq_mkAtom, [|p|])
+      | AtomProp (p, Some prf) ->
+        EConstr.mkApp (Lazy.force coq_mkAtomDec, [|p; prf|])
+      | AtomBool (b, p, prf) ->
+        EConstr.mkApp (Lazy.force coq_TBool, [|b; p; prf|])
     in
     let add i e m =
       EConstr.mkApp (add, [|ty; EConstr.mkInt (Uint63.of_int i); mk_atom e; m|])
@@ -168,56 +316,96 @@ module Env = struct
     let rec map_of_list l =
       match l with
       | [] -> EConstr.mkApp (Lazy.force coq_empty, [|ty|])
-      | (e, (i, d)) :: l -> add i (e, d) (map_of_list l)
+      | (e, i) :: l -> add i e (map_of_list l)
     in
     map_of_list env.vars
 end
 
 let hcons i b f = P.HCons.{id = Uint63.of_int i; is_dec = b; elt = f}
 
-let reify_formula genv env (f : EConstr.t) =
+let reify_formula genv env k (f : EConstr.t) =
   let evd = env.Env.sigma in
-  let tt = hcons 1 true P.TT in
-  let ff = hcons 0 true P.FF in
-  let mkop o f1 f2 = P.OP (o, f1, f2) in
+  let tt k = hcons 1 true (P.BForm.BTT k) in
+  let ff k = hcons 0 true (P.BForm.BFF k) in
+  let mkop k o f1 f2 = P.BForm.BOP (k, o, f1, f2) in
   let eq_ind r i = GlobRef.equal r (GlobRef.IndRef i) in
-  let is_true = eq_ind (Lazy.force coq_True) in
-  let is_false = eq_ind (Lazy.force coq_False) in
+  let eq_constructor r c = GlobRef.equal r (GlobRef.ConstructRef c) in
+  let eq_const r c = GlobRef.equal r (GlobRef.ConstRef c) in
+  let is_True = eq_ind (Lazy.force coq_True) in
+  let is_False = eq_ind (Lazy.force coq_False) in
   let is_and = eq_ind (Lazy.force coq_and) in
   let is_or = eq_ind (Lazy.force coq_or) in
-  let var env f =
-    let env', (i, dec) = Env.hcons_atom genv env f in
-    (hcons i (Env.is_dec dec) (P.AT (Uint63.of_int i)), env')
+  let is_andb = eq_const (Lazy.force coq_andb) in
+  let is_orb = eq_const (Lazy.force coq_orb) in
+  let is_implb = eq_const (Lazy.force coq_implb) in
+  let is_is_True = eq_const (Lazy.force coq_Is_true) in
+  let is_true = eq_constructor (Lazy.force coq_true) in
+  let is_false = eq_constructor (Lazy.force coq_false) in
+  let var env k f =
+    let env', (atom, i) = Env.hcons_atom genv env k f in
+    (hcons i (Env.is_dec atom) (P.BForm.BAT (k, Uint63.of_int i)), env')
   in
-  let get_binop t =
-    match EConstr.kind evd t with
-    | Ind (i, _) ->
-      if is_and i then P.AND else if is_or i then P.OR else raise Not_found
-    | _ -> raise Not_found
+  let get_binop k t =
+    match k with
+    | P.IsProp -> (
+      match EConstr.kind evd t with
+      | Ind (i, _) ->
+        if is_and i then P.AND else if is_or i then P.OR else raise Not_found
+      | _ -> raise Not_found )
+    | P.IsBool -> (
+      match EConstr.kind evd t with
+      | Const (c, _) ->
+        if is_andb c then P.AND
+        else if is_orb c then P.OR
+        else if is_implb c then P.IMPL
+        else raise Not_found
+      | _ -> raise Not_found )
   in
-  let rec reify_formula env f =
+  let rec reify_formula env k f =
     match EConstr.kind evd f with
-    | Ind (i, _) ->
-      if is_true i then (tt, env)
-      else if is_false i then (ff, env)
-      else var env f
+    | Ind (i, _) -> (
+      match k with
+      | P.IsProp ->
+        if is_True i then (tt k, env)
+        else if is_False i then (ff k, env)
+        else var env k f
+      | P.IsBool -> var env k f )
+    | Construct (c, _) ->
+      if is_true c then (tt P.IsBool, env)
+      else if is_false c then (ff P.IsBool, env)
+      else var env k f
     | App (h, [|f1; f2|]) -> (
       try
-        let op = get_binop h in
-        let f1, env = reify_formula env f1 in
-        let f2, env = reify_formula env f2 in
+        let op = get_binop k h in
+        let f1, env = reify_formula env k f1 in
+        let f2, env = reify_formula env k f2 in
         let env, i = Env.hcons_op env op f1.P.HCons.id f2.P.HCons.id in
-        (hcons i (f1.P.HCons.is_dec && f2.P.HCons.is_dec) (mkop op f1 f2), env)
-      with Not_found -> var env f )
+        (hcons i (f1.P.HCons.is_dec && f2.P.HCons.is_dec) (mkop k op f1 f2), env)
+      with Not_found -> var env k f )
     | Prod (t, f1, f2)
       when t.Context.binder_name = Anonymous || EConstr.Vars.noccurn evd 1 f2 ->
-      let f1, env = reify_formula env f1 in
-      let f2, env = reify_formula env f2 in
+      let f1, env = reify_formula env P.IsProp f1 in
+      let f2, env = reify_formula env P.IsProp f2 in
       let env, i = Env.hcons_op env P.IMPL f1.P.HCons.id f2.P.HCons.id in
-      (hcons i (f1.P.HCons.is_dec && f2.P.HCons.is_dec) (mkop P.IMPL f1 f2), env)
-    | _ -> var env f
+      ( hcons i
+          (f1.P.HCons.is_dec && f2.P.HCons.is_dec)
+          (mkop P.IsProp P.IMPL f1 f2)
+      , env )
+    | App (h, [|f1|]) -> (
+      match k with
+      | P.IsBool -> var env k f
+      | P.IsProp -> (
+        match EConstr.kind evd h with
+        | Const (c, _) ->
+          if is_is_True c then
+            let f1, env = reify_formula env P.IsBool f1 in
+            ( hcons (Uint63.hash f1.P.HCons.id) true (P.BForm.BIT f1.P.HCons.elt)
+            , env )
+          else var env k f
+        | _ -> var env k f ) )
+    | _ -> var env k f
   in
-  reify_formula env f
+  reify_formula env k f
 
 let rec reify_hyps genv env (hyps : (Names.Id.t * EConstr.types) list) =
   match hyps with
@@ -225,13 +413,13 @@ let rec reify_hyps genv env (hyps : (Names.Id.t * EConstr.types) list) =
   | (id, t) :: l ->
     let lhyps, env = reify_hyps genv env l in
     if is_prop genv env.Env.sigma t then
-      let hf, env = reify_formula genv env t in
+      let hf, env = reify_formula genv env P.IsProp t in
       ((id, hf) :: lhyps, env)
     else (lhyps, env)
 
 let reify_goal genv env hyps concl =
   let hyps, env = reify_hyps genv env hyps in
-  let hf, env = reify_formula genv env concl in
+  let hf, env = reify_formula genv env P.IsProp concl in
   (hyps, hf, env)
 
 let make_formula env hyps hconcl =
@@ -242,13 +430,13 @@ let make_formula env hyps hconcl =
       let hf2, env = make env hyps hconcl in
       let env, i = Env.hcons_op env P.IMPL hf1.P.HCons.id hf2.P.HCons.id in
       let is_dec = hf1.P.HCons.is_dec && hf2.P.HCons.is_dec in
-      (hcons i is_dec (P.OP (P.IMPL, hf1, hf2)), env)
+      (hcons i is_dec (P.BForm.BOP (P.IsProp, P.IMPL, hf1, hf2)), env)
   in
   make env hyps hconcl
 
 let constr_of_bool = function
-  | true -> Lazy.force coq_true
-  | false -> Lazy.force coq_false
+  | true -> constr_of_gref (Lazy.force coq_true)
+  | false -> constr_of_gref (Lazy.force coq_false)
 
 let hc typ i b v =
   EConstr.mkApp
@@ -311,6 +499,35 @@ let constr_of_formula f =
     in
     constr_of_hcons ftyp constr_of_op_formula f)
 
+let constr_of_kind = function
+  | P.IsProp -> Lazy.force coq_IsProp
+  | P.IsBool -> Lazy.force coq_IsBool
+
+let constr_of_bformula f =
+  let tt k = EConstr.mkApp (Lazy.force coq_BTT, [|constr_of_kind k|]) in
+  let ff k = EConstr.mkApp (Lazy.force coq_BFF, [|constr_of_kind k|]) in
+  let ftyp k = EConstr.mkApp (Lazy.force coq_BFormula, [|constr_of_kind k|]) in
+  let at k i =
+    EConstr.mkApp (Lazy.force coq_BAT, [|constr_of_kind k; EConstr.mkInt i|])
+  in
+  let mk_op = Lazy.force coq_BOP in
+  let mkop k o f1 f2 =
+    EConstr.mkApp (mk_op, [|constr_of_kind k; constr_of_op o; f1; f2|])
+  in
+  P.BForm.(
+    let rec constr_of_op_formula f =
+      match f with
+      | BTT k -> tt k
+      | BFF k -> ff k
+      | BAT (k, i) -> at k i
+      | BOP (k, o, f1, f2) ->
+        mkop k o
+          (constr_of_hcons (ftyp k) constr_of_op_formula f1)
+          (constr_of_hcons (ftyp k) constr_of_op_formula f2)
+      | BIT f -> EConstr.mkApp (Lazy.force coq_BIT, [|constr_of_op_formula f|])
+    in
+    constr_of_hcons (ftyp P.IsProp) constr_of_op_formula f)
+
 let nat_of_int i =
   if i < 0 then P.O
   else
@@ -319,105 +536,157 @@ let nat_of_int i =
 
 module Theory = struct
   open ProverPatch
-  open Micromega_plugin
-  module Mc = Micromega
 
-  let rec parse_clause (genv, sigma) ep env l =
-    match l with
-    | [] -> (Mc.FF Mc.IsProp, env)
-    | a :: l -> (
-      let f, env = parse_clause (genv, sigma) ep env l in
-      try
-        let form = form_of_literal a in
-        let eform, i = Env.get_constr_of_atom ep form in
-        let at, env =
-          Coq_micromega.parse_zarith Mc.IsProp env eform (genv, sigma)
-        in
-        let at = Mc.A (Mc.IsProp, at, i) in
-        match a with
-        | POS _ -> (Mc.OR (Mc.IsProp, at, f), env)
-        | NEG _ -> (Mc.IMPL (Mc.IsProp, at, None, f), env)
-      with Not_found | Coq_micromega.ParseError | Failure _ -> (f, env) )
-
-  open Coq_micromega
-  open Certificate
-
-  let iset_of_list l =
-    List.fold_left (fun acc i -> Mutils.ISet.add i acc) Mutils.ISet.empty l
-
-  let map_of_list l =
-    let rec map_of_list m i l =
+  let split_clause l =
+    let rec split_acc ln lp l =
       match l with
-      | [] -> m
-      | (_, id) :: l -> map_of_list (IMap.add i id m) (i + 1) l
+      | [] -> (ln, lp)
+      | at :: l -> (
+        match at with
+        | NEG _ -> split_acc (at :: ln) lp l
+        | POS _ -> split_acc ln (at :: lp) l )
     in
-    map_of_list IMap.empty 0 l
+    split_acc [] [] l
 
-  let find_deps_of_prf p prf l =
-    let m = map_of_list l in
-    let hyps = p.hyps prf in
-    Mutils.ISet.fold
-      (fun i acc -> Mutils.ISet.add (IMap.find i m) acc)
-      hyps Mutils.ISet.empty
+  let id_of_literal a =
+    Names.Id.of_string_soft
+      ("cid__" ^ string_of_int (Uint63.hash (id_of_literal a)))
 
-  let find_unsat_clause p clid =
-    let cl = List.map fst clid in
-    match p.prover (p.get_option (), cl) with
-    | Model _ -> None
-    | Unknown -> None
-    | Prf prf -> Some (find_deps_of_prf p prf clid)
+  let rec constr_of_clause ep cl =
+    match cl with
+    | [] -> constr_of_gref (Lazy.force coq_False)
+    | a :: l -> (
+      let c = constr_of_clause ep l in
+      let at = fst (Env.get_constr_of_atom ep (form_of_literal a)) in
+      match a with
+      | NEG _ -> EConstr.mkProd (Context.nameR (id_of_literal a), at, c)
+      | POS _ -> (
+        match l with
+        | [] -> at
+        | _ -> EConstr.mkApp (constr_of_gref (Lazy.force coq_or), [|at; c|]) ) )
 
-  let rec find_unsat_core p s l =
-    match l with
-    | [] -> Some s
-    | cl :: l -> (
-      match find_unsat_clause p cl with
-      | None -> None
-      | Some s' -> find_unsat_core p (Mutils.ISet.union s s') l )
+  let name_of_binder c =
+    match Context.binder_name c with
+    | Name.Anonymous -> raise Not_found
+    | Name.Name id -> id
 
-  let select_atom is lit =
-    let id = Uint63.hash (form_of_literal lit).HCons.id in
-    Mutils.ISet.mem id is
+  let rec intros_proof evd binders c =
+    match EConstr.kind evd c with
+    | Lambda (c, _, t) -> intros_proof evd (name_of_binder c :: binders) t
+    | _ -> (binders, c)
 
-  let thy_prover cc p (genv, sigma) ep hm l =
-    let env = Coq_micromega.Env.empty (genv, sigma) in
-    let cl, _ = parse_clause (genv, sigma) ep env l in
-    let cnf_ff, cnf_ff_tags = Mc.cnfZ Mc.IsProp cl in
-    match find_unsat_core p (iset_of_list cnf_ff_tags) cnf_ff with
-    | None ->
-      Printf.fprintf stdout "Thy ⊬ %a\n" P.output_literal_list l;
-      None
-    | Some is ->
-      let c = List.filter (select_atom is) l in
-      Printf.fprintf stdout "Thy ⊢ %a\n" P.output_literal_list c;
-      cc := c :: !cc;
-      Some (hm, c)
+  module ISet = Set.Make (Int)
+
+  let hyps_of_rels s l =
+    let rec select i l =
+      match l with
+      | [] -> []
+      | e :: l ->
+        if ISet.mem i s then e :: select (i + 1) l else select (i + 1) l
+    in
+    select 1 l
+
+  let deps_of_proof evd c =
+    let rec deps d s c =
+      match EConstr.kind evd c with
+      | Rel i ->
+        let i' = i - d in
+        if i' <= 0 then s else ISet.add i' s
+      | App (c, i) -> Array.fold_left (fun s t -> deps d s t) (deps d s c) i
+      | Const _ | Construct _ | Var _ | Sort _ | Ind _ -> s
+      | Lambda (x, t, e) -> deps (d + 1) (deps d s t) e
+      | Prod (x, t, e) -> deps (d + 1) (deps d s t) e
+      | LetIn (x, e1, t1, e2) -> deps (d + 1) (deps d (deps d s e1) t1) e2
+      | Cast (c, _, t) -> deps d (deps d s c) t
+      | Int _ | Float _ -> s
+      | _ ->
+        Feedback.msg_debug
+          Pp.(str "deps_of_proof : " ++ pr_constr (Global.env ()) evd c);
+        failwith "deps of proof"
+    in
+    let binders, prf = intros_proof evd [] c in
+    hyps_of_rels (deps 0 ISet.empty prf) binders
+
+  let rec concl_of_clause cl =
+    match cl with
+    | [] -> []
+    | at :: l -> ( match at with NEG _ -> concl_of_clause l | POS _ -> cl )
+
+  let rec get_used_hyps l' cl =
+    match l' with
+    | [] -> concl_of_clause cl
+    | e :: l' -> (
+      match cl with
+      | [] -> failwith "get_used_hyps"
+      | at :: cl ->
+        if Names.Id.equal e (id_of_literal at) then at :: get_used_hyps l' cl
+        else get_used_hyps (e :: l') cl )
+
+  type 'a core = UnsatCore of P.literal list | NoCore of 'a
+
+  let find_unsat_core ep cl tac env sigma =
+    let gl = constr_of_clause ep cl in
+    let e, pv = Proofview.init sigma [(env, gl)] in
+    try
+      let _, pv, _, _ =
+        Proofview.apply
+          ~name:(Names.Id.of_string "unsat_core")
+          ~poly:false env
+          (Tacticals.New.tclTHEN (Tactics.keep [])
+             (Tacticals.New.tclCOMPLETE tac))
+          pv
+      in
+      match Proofview.partial_proof e pv with
+      | [prf] ->
+        let l = List.rev (deps_of_proof sigma prf) in
+        UnsatCore (get_used_hyps l cl)
+      | _ -> failwith "Multiple proof terms"
+    with e when CErrors.noncritical e -> NoCore (CErrors.print e, gl)
+
+  let find_unsat_core ep cl tac env sigma =
+    let ln, lp = split_clause cl in
+    let rec all_cores c =
+      match c with
+      | [] -> NoCore []
+      | c1 :: c -> (
+        match find_unsat_core ep (ln @ [c1]) tac env sigma with
+        | UnsatCore s -> UnsatCore s
+        | NoCore r -> (
+          match all_cores c with
+          | UnsatCore s -> UnsatCore s
+          | NoCore r' -> NoCore (r :: r') ) )
+    in
+    match find_unsat_core ep lp tac env sigma with
+    | NoCore _ -> all_cores lp
+    | UnsatCore s -> UnsatCore s
+
+  let pp_no_core env sigma l =
+    Pp.(
+      pr_enum
+        (fun (fail, gl) -> fail ++ str " for " ++ pr_constr env sigma gl)
+        l)
+
+  let thy_prover tac cc p (genv, sigma) ep hm l =
+    match find_unsat_core ep l tac genv sigma with
+    | NoCore r -> CErrors.user_err (pp_no_core genv sigma r)
+    | UnsatCore core ->
+      Printf.fprintf stdout "Thy ⊢ %a\n" P.output_literal_list core;
+      cc := core :: !cc;
+      Some (hm, core)
 end
 
-let run_prover cc (genv, sigma) ep f =
+let run_prover tac cc (genv, sigma) ep f =
   let is_dec i =
     try
-      let c, d = Env.AMap.find (Uint63.hash i) ep.Env.amap in
+      let d = Env.AMap.find (Uint63.hash i) ep.Env.amap in
       Env.is_dec d
     with Not_found -> false
   in
   let m = P.hcons_form f in
   P.prover_formula is_dec
-    (Theory.thy_prover cc Micromega_plugin.Coq_micromega.linear_Z (genv, sigma)
-       ep)
+    (Theory.thy_prover tac cc Micromega_plugin.Coq_micromega.linear_Z
+       (genv, sigma) ep)
     true m (nat_of_int 200) f
-
-let constr_of_literal_list ep mkFF mkOr mkImpl l =
-  P.(
-    let rec constr_of_literal_list l =
-      match l with
-      | [] -> mkFF
-      | x :: l ->
-        (match x with POS a -> mkOr | NEG a -> mkImpl)
-          (fst (Env.get_constr_of_atom ep (P.form_of_literal x)))
-          (constr_of_literal_list l)
-    in
-    constr_of_literal_list l)
 
 let fresh_id id gl =
   Tactics.fresh_id_in_env Id.Set.empty id (Proofview.Goal.env gl)
@@ -434,15 +703,12 @@ let fresh_id id gl =
  *)
 
 let assert_conflicts ep l tac gl =
-  let mkFF = constr_of_gref (Lazy.force coq_False) in
-  let mkOr x y = EConstr.mkApp (constr_of_gref (Lazy.force coq_or), [|x; y|]) in
-  let mkImpl x y = EConstr.mkArrow x Sorts.Irrelevant y in
-  let mk_goal c = constr_of_literal_list ep mkFF mkOr mkImpl c in
+  let mk_goal c = Theory.constr_of_clause ep c in
   let rec assert_conflicts n l =
     match l with
     | [] -> Tacticals.New.tclIDTAC
     | c :: l ->
-      let id = fresh_id (Names.Id.of_string ("__arith" ^ string_of_int n)) gl in
+      let id = fresh_id (Names.Id.of_string ("__cc" ^ string_of_int n)) gl in
       Tacticals.New.tclTHEN
         (Tactics.assert_by (Names.Name id) (mk_goal c)
            (Tacticals.New.tclTHEN (Tactics.keep []) tac))
@@ -460,9 +726,16 @@ let assert_conflicts_clauses tac =
       let concl = Tacmach.New.pf_concl gl in
       let hyps = Tacmach.New.pf_hyps_types gl in
       let hyps, concl, env = reify_goal genv (Env.empty sigma) hyps concl in
-      let form, env = make_formula env (List.rev hyps) concl in
+      let bform, env = make_formula env (List.rev hyps) concl in
+      let has_bool i =
+        try
+          let d = Env.AMap.find (Uint63.hash i) env.Env.amap in
+          Env.has_bool d
+        with Not_found -> false
+      in
+      let form = P.BForm.to_hformula has_bool bform in
       let cc = ref [] in
-      match run_prover cc (genv, sigma) env form with
+      match run_prover tac cc (genv, sigma) env form with
       | P.HasProof _ -> assert_conflicts env !cc tac gl
       | _ -> Tacticals.New.tclFAIL 0 (Pp.str "Not a tautology"))
 
@@ -475,14 +748,34 @@ let change_goal =
       let hyps = Tacmach.New.pf_hyps_types gl in
       let hyps, concl, env = reify_goal genv (Env.empty sigma) hyps concl in
       let form, env = make_formula env (List.rev hyps) concl in
-      let cform = constr_of_formula form in
+      let cform = constr_of_bformula form in
       let m = Env.map_of_env env in
-      Tacticals.New.tclTHEN
-        (Tactics.generalize
-           (List.rev_map (fun x -> EConstr.mkVar (fst x)) hyps))
-        (Tactics.change_concl
-           (EConstr.mkApp
-              ( Lazy.force coq_eval_hformula
-              , [|EConstr.mkApp (Lazy.force coq_eval_prop, [|m|]); cform|] ))))
+      let change =
+        EConstr.mkApp
+          ( Lazy.force coq_eval_hbformula
+          , [|EConstr.mkApp (Lazy.force coq_eval_prop, [|m|]); cform|] )
+      in
+      Tacticals.New.tclOR
+        (Tacticals.New.tclTHEN
+           (Tactics.generalize
+              (List.rev_map (fun x -> EConstr.mkVar (fst x)) hyps))
+           (Tactics.change_concl change))
+        (Tacticals.New.tclFAIL 0 (pr_constr genv sigma change)))
+
+let is_loaded_library d =
+  let make_dir l = DirPath.make (List.rev_map Id.of_string l) in
+  let dir = make_dir d in
+  try
+    let (_ : Declarations.module_body) =
+      Global.lookup_module (ModPath.MPfile dir)
+    in
+    true
+  with Not_found -> false
+
+let nnpp =
+  Proofview.Goal.enter (fun gl ->
+      if is_loaded_library ["Coq"; "Logic"; "Classical_Prop"] then
+        Tactics.apply (Lazy.force coq_nnpp)
+      else Tacticals.New.tclIDTAC)
 
 let cdcl tac = Tacticals.New.tclTHEN (assert_conflicts_clauses tac) change_goal
