src/ppprover.ml
@@ -1,0 +1,177 @@
+open Prover
+
+(** val empty_state *)
+
+let string_op = function AND -> "∧" | OR -> "∨" | IMPL -> "→"
+
+let rec output_formula o = function
+  | TT -> output_string o "⊤"
+  | FF -> output_string o "⊥"
+  | AT i -> Printf.fprintf o "p%i" (Uint63.hash i)
+  | OP (op, f1, f2) ->
+    Printf.fprintf o "(%a %s %a)" output_formula f1.HCons.elt (string_op op)
+      output_formula f2.HCons.elt
+
+let output_lit o = function
+  | POS p -> Printf.fprintf o "[%a]" output_formula p.HCons.elt
+  | NEG p -> Printf.fprintf o "~[%a]" output_formula p.HCons.elt
+
+let output_hform o f = Printf.fprintf o "%a" output_formula f.HCons.elt
+
+let output_oform o f =
+  match f with None -> output_string o "⊥" | Some f -> output_hform o f
+
+let rec output_literal_list o l =
+  match l with
+  | [] -> output_string o "⊥"
+  | [POS p] -> Printf.fprintf o "[%a]" output_formula p.HCons.elt
+  | POS p :: l ->
+    Printf.fprintf o "[%a] ∨ %a" output_formula p.HCons.elt
+      output_literal_list l
+  | NEG p :: l ->
+    Printf.fprintf o "[%a] → %a" output_formula p.HCons.elt
+      output_literal_list l
+
+let output_watched_clause o l =
+  output_literal_list o (l.watch1 :: l.watch2 :: l.unwatched)
+
+let rec unprovable l =
+  match l with
+  | [] -> false
+  | NEG f :: l -> f.HCons.elt = FF || unprovable l
+  | POS f :: l -> false
+
+let output_useful_watched_clause o l =
+  let l = l.watch1 :: l.watch2 :: l.unwatched in
+  if unprovable l then () else output_literal_list o l
+
+let output_clause o = function
+  | EMPTY -> output_string o "⊥"
+  | TRUE -> output_string o "⊤"
+  | UNIT r -> output_lit o r
+  | CLAUSE l -> output_watched_clause o l
+
+let rec output_list out o l =
+  match l with
+  | [] -> ()
+  | [e] -> out o e
+  | e :: l -> out o e; output_string o ";"; output_list out o l
+
+let output_map out o m =
+  IntMap.fold' (fun _ i cl -> Printf.fprintf o "%a;" out cl) m ()
+
+let output_clauses o m =
+  IntMap.fold'
+    (fun _ i (m1, m2) ->
+      output_map output_useful_watched_clause o m1;
+      output_map output_useful_watched_clause o m2)
+    m ()
+
+let output_units hm o m =
+  let out_elt i b =
+    match IntMap.get' kInt i hm with
+    | None -> failwith "Unknow literal"
+    | Some (b', f) ->
+      let hf = HCons.{id = i; is_dec = b'; elt = f} in
+      Printf.fprintf o "%i:%a;" (Uint63.hash i) output_lit
+        (if b then POS hf else NEG hf)
+  in
+  IntMap.fold' (fun _ i b -> out_elt i b) m ()
+
+let output_wneg hm o m =
+  let out_elt i b =
+    match IntMap.get' kInt i hm with
+    | None -> failwith "Unknow literal"
+    | Some (b', f) ->
+      let hf = HCons.{id = i; is_dec = b'; elt = f} in
+      Printf.fprintf o "%i:%a;" (Uint63.hash i) output_hform hf
+  in
+  IntMap.fold' (fun _ i b -> out_elt i b) m ()
+
+let output_state o st =
+  Printf.fprintf o "Arrows : %a\n" (output_list output_lit) st.arrows;
+  Printf.fprintf o "WNEG : %a\n" (output_wneg st.hconsmap) st.wneg;
+  Printf.fprintf o "Lit : %a\n" (output_list output_lit) st.unit_stack;
+  Printf.fprintf o "Units : %a\n" (output_units st.hconsmap) st.units;
+  Printf.fprintf o "Clauses : %a\n" output_clauses st.clauses
+
+(**  *)
+
+(** *)
+let cnf pol is_classic cp cm ar acc f hf =
+  let x, cl = cnf pol is_classic cp cm ar acc f hf in
+  Printf.printf "cnf %a ⊢ %a\n" output_formula f
+    (output_list output_useful_watched_clause)
+    cl;
+  (x, cl)
+
+(** *)
+let reduce lit cl =
+  let res = reduce lit cl in
+  ( match res with
+  | None -> Printf.printf "reduce : %a -> ∅\n" output_literal_list cl
+  | Some r ->
+    Printf.printf "reduce : %a -> %a\n" output_literal_list cl
+      output_literal_list r );
+  res
+
+(** *)
+
+let cnf_hyps b hs st =
+  Printf.printf "cnf_hyps: %a\n" output_literal_list hs;
+  cnf_hyps b hs st
+
+(** *)
+
+let intro_state st f hf =
+  match intro_state st f hf with
+  | None ->
+    Printf.printf "intro state ⊢ ⊥ \n";
+    None
+  | Some (st', g) ->
+    Printf.printf "intro state ⊢\n%a\n" output_state st';
+    Some (st', g)
+
+(** *)
+
+let unit_propagation n st concl =
+  let res = unit_propagation n st concl in
+  ( match res with
+  | Success -> Printf.printf "OK"
+  | OutOfFuel -> Printf.printf "KO"
+  | Progress st -> Printf.printf "unit_propagation ⊢\n%a\n" output_state st );
+  res
+
+(** *)
+let select_clause b l acc k cl =
+  let res = select_clause b l acc k cl in
+  ( match (acc, res) with
+  | _, Some l ->
+    Printf.printf "select_clause %a -> %a\n" output_watched_clause cl
+      output_literal_list l
+  | _, _ -> Printf.printf "select_clause %a -> ∅ \n" output_watched_clause cl
+  );
+  res
+
+(** *)
+let find_split lit is_bot cl =
+  let res = find_split lit is_bot cl in
+  ( match res with
+  | None -> Printf.printf "find_split  -> ∅\n"
+  | Some l -> Printf.printf "find_split  -> %a\n" (output_list output_lit) l );
+  res
+
+(** *)
+let find_arrows st l =
+  let res = find_arrows st l in
+  Printf.printf "find_arrows %a -> %a\n" (output_list output_lit) l
+    (output_list output_lit) res;
+  res
+(** *)
+
+let prover_intro p st g =
+  let res = prover_intro p st g in
+  ( match res with
+  | HasProof _ -> Printf.fprintf stdout "prover ⊢ %a\n" output_oform g
+  | _ -> Printf.fprintf stdout "prover ⊬ %a\n" output_oform g );
+  flush stdout; res
